ironfleet/src/Dafny/Distributed/Protocol/Lock/RefinementProof/RefinementProof.i.dfy
@@ -9,63 +9,72 @@ module RefinementProof_i {
     import opened Collections__Maps_i
     import opened Logic__Option_i
 
-    lemma lemma_InitRefines(ls:LS_State, config:Config) 
-        requires LS_Init(ls, config);
-        ensures  Service_Init(AbstractifyLS_State(ls), UniqueSeqToSet(config));
+    lemma lemma_InitRefines(gls:GLS_State, config:Config) 
+        requires GLS_Init(gls, config);
+        ensures  Service_Init(AbstractifyGLS_State(gls), UniqueSeqToSet(config));
     {
         assert config[0] in config; // OBSERVE: triggers the exists in Service_Init
+        var s := AbstractifyGLS_State(gls);
+        calc {
+            s.hosts;
+            mapdomain(gls.ls.servers);
+            UniqueSeqToSet(config);
+        }
+
+        assert config[0] in config; // OBSERVE
+        assert config[0] in UniqueSeqToSet(config);
     }
 
-    predicate IsValidBehavior(lb:seq<LS_State>, config:Config)
+    predicate IsValidBehavior(glb:seq<GLS_State>, config:Config)
     {
-        |lb| > 0
-     && LS_Init(lb[0], config)
-     && (forall i :: 0 <= i < |lb| - 1 ==> LS_Next(lb[i], lb[i+1]))
+        |glb| > 0
+     && GLS_Init(glb[0], config)
+     && (forall i :: 0 <= i < |glb| - 1 ==> GLS_Next(glb[i], glb[i+1]))
     }
 
-    lemma lemma_LS_Next(lb:seq<LS_State>, config:Config, i:int)
-        requires IsValidBehavior(lb, config);
-        requires 0 <= i < |lb| - 1;
-        ensures  LS_Next(lb[i], lb[i+1]);
+    lemma lemma_LS_Next(glb:seq<GLS_State>, config:Config, i:int)
+        requires IsValidBehavior(glb, config);
+        requires 0 <= i < |glb| - 1;
+        ensures  GLS_Next(glb[i], glb[i+1]);
     {
     }
 
-    lemma lemma_LSConsistent(lb:seq<LS_State>, config:Config, i:int)
-        requires IsValidBehavior(lb, config);
-        requires 0 <= i < |lb|;
-        ensures  |lb[i].servers| == |config|;
-        ensures  forall e :: e in config <==> e in lb[i].servers;
-        ensures  mapdomain(lb[i].servers) == mapdomain(lb[0].servers);
-        ensures  forall id :: id in config ==> lb[0].servers[id].config == lb[i].servers[id].config;
+    lemma lemma_LSConsistent(glb:seq<GLS_State>, config:Config, i:int)
+        requires IsValidBehavior(glb, config);
+        requires 0 <= i < |glb|;
+        ensures  |glb[i].ls.servers| == |config|;
+        ensures  forall e :: e in config <==> e in glb[i].ls.servers;
+        ensures  mapdomain(glb[i].ls.servers) == mapdomain(glb[0].ls.servers);
+        ensures  forall id :: id in config ==> glb[0].ls.servers[id].config == glb[i].ls.servers[id].config;
     {
         if i == 0 {
             calc {
                 UniqueSeqToSet(config);
-                mapdomain(lb[0].servers);
+                mapdomain(glb[0].ls.servers);
             }
-            lemma_seqs_set_cardinality(config, mapdomain(lb[0].servers));
+            lemma_seqs_set_cardinality(config, mapdomain(glb[0].ls.servers));
             calc {
-                |mapdomain(lb[0].servers)|;
-                    { lemma_MapSizeIsDomainSize(mapdomain(lb[0].servers), lb[0].servers); }
-                |lb[0].servers|;
+                |mapdomain(glb[0].ls.servers)|;
+                    { lemma_MapSizeIsDomainSize(mapdomain(glb[0].ls.servers), glb[0].ls.servers); }
+                |glb[0].ls.servers|;
             }
         } else {
-            lemma_LS_Next(lb, config, i - 1);
-            lemma_LSConsistent(lb, config, i - 1);
+            lemma_LS_Next(glb, config, i - 1);
+            lemma_LSConsistent(glb, config, i - 1);
         }
     }
 
-    lemma lemma_LSNodeConsistent(lb:seq<LS_State>, config:Config, i:int, candidate:EndPoint, e:EndPoint)
-        requires IsValidBehavior(lb, config);
-        requires 0 <= i < |lb|;
-        requires e in lb[i].servers;
-        ensures  candidate in lb[i].servers <==> candidate in lb[i].servers[e].config;
+    lemma lemma_LSNodeConsistent(glb:seq<GLS_State>, config:Config, i:int, candidate:EndPoint, e:EndPoint)
+        requires IsValidBehavior(glb, config);
+        requires 0 <= i < |glb|;
+        requires e in glb[i].ls.servers;
+        ensures  candidate in glb[i].ls.servers <==> candidate in glb[i].ls.servers[e].config;
     {
         if i == 0 {
         } else {
-            lemma_LS_Next(lb, config, i-1);
-            lemma_LSConsistent(lb, config, i-1);
-            lemma_LSNodeConsistent(lb, config, i-1, candidate, e);
+            lemma_LS_Next(glb, config, i-1);
+            lemma_LSConsistent(glb, config, i-1);
+            lemma_LSNodeConsistent(glb, config, i-1, candidate, e);
         }
     }
 
@@ -93,68 +102,79 @@ module RefinementProof_i {
         }
     }
 
-    */
+    
 
+    predicate ExistsLockPacket(glb:seq<GLS_State>, config:Config, i:int, j:int)
+        requires IsValidBehavior(glb, config);
+        requires 0 <= i < |glb|-1;
+    {
+        exists p :: p in glb[i].ls.environment.sentPackets && p.msg.Locked? && p.msg.locked_epoch == j
+    }*/
 
-    lemma lemma_HistoryIncrement(lb:seq<LS_State>, config:Config, i:int)
-        requires IsValidBehavior(lb, config);
-        requires 0 <= i < |lb| - 1;
-        ensures  |lb[i].history| + 1 == |lb[i+1].history|
-              || lb[i].history == lb[i+1].history;
+    
+    lemma lemma_HistoryIncrement(glb:seq<GLS_State>, config:Config, i:int)
+        requires IsValidBehavior(glb, config);
+        requires 0 <= i < |glb| - 1;
+        ensures  |glb[i].history| + 1 == |glb[i].history|
+              || glb[i].history == glb[i].history;
     { }
 
-    lemma lemma_HistorySize(lb:seq<LS_State>, config:Config, i:int)
-        requires IsValidBehavior(lb, config);
-        requires 0 <= i < |lb|;
-        ensures  1 <= |lb[i].history| <= i + 1;
+    lemma lemma_HistorySize(glb:seq<GLS_State>, config:Config, i:int)
+        requires IsValidBehavior(glb, config);
+        requires 0 <= i < |glb|;
+        ensures  1 <= |glb[i].history| <= i + 1;
     { 
         if i == 0 {
+            var locked_packets := set p | p in glb[i].ls.environment.sentPackets && p.msg.Locked?;
+            assert |locked_packets| == 0;
+            assert exists host :: host in (glb[i]).ls.servers && (glb[i]).ls.servers[host].held;
+            assert |glb[i].history| == 1;
         } else {
-            lemma_HistorySize(lb, config, i - 1);
-            lemma_HistoryIncrement(lb, config, i - 1);
+            lemma_HistorySize(glb, config, i - 1);
+            lemma_HistoryIncrement(glb, config, i - 1);
         }
     }
 
-    lemma lemma_HistoryMembership(lb:seq<LS_State>, config:Config, i:int)
-        requires IsValidBehavior(lb, config);
-        requires 0 <= i < |lb|;
-        ensures  1 <= |lb[i].history| <= i + 1;
-        ensures  last(lb[i].history) in lb[i].servers;
+    lemma lemma_HistoryMembership(glb:seq<GLS_State>, config:Config, i:int)
+        requires IsValidBehavior(glb, config);
+        requires 0 <= i < |glb|;
+        ensures  1 <= |glb[i].history| <= i + 1;
+        ensures  last(glb[i].history) in glb[i].ls.servers;
     {
-        lemma_HistorySize(lb, config, i);
+        lemma_HistorySize(glb, config, i);
 
         if i == 0 { 
         } else {
-            lemma_LS_Next(lb, config, i - 1);
-            lemma_LSConsistent(lb, config, i - 1);
-            lemma_LSConsistent(lb, config, i);
-            lemma_HistoryMembership(lb, config, i-1);
+            lemma_LS_Next(glb, config, i - 1);
+            lemma_LSConsistent(glb, config, i - 1);
+            lemma_LSConsistent(glb, config, i);
+            lemma_HistoryMembership(glb, config, i-1);
         }
     }
 
-    lemma lemma_LS_NextAbstract(lb:seq<LS_State>, config:Config, i:int)
-        requires IsValidBehavior(lb, config);
-        requires 0 <= i < |lb| - 1;
-        ensures  ServiceNext(AbstractifyLS_State(lb[i]), AbstractifyLS_State(lb[i+1]))
-               || AbstractifyLS_State(lb[i]) == AbstractifyLS_State(lb[i+1]);
+    lemma lemma_LS_NextAbstract(glb:seq<GLS_State>, config:Config, i:int)
+        requires IsValidBehavior(glb, config);
+        requires 0 <= i < |glb| - 1;
+        ensures  ServiceNext(AbstractifyGLS_State(glb[i]), AbstractifyGLS_State(glb[i+1]))
+               || AbstractifyGLS_State(glb[i]) == AbstractifyGLS_State(glb[i+1]);
     {
-        lemma_LSConsistent(lb, config, i);
-        lemma_LSConsistent(lb, config, i+1);
+        lemma_LSConsistent(glb, config, i);
+        lemma_LSConsistent(glb, config, i+1);
 
         if i == 0 {
-            assert lb[i].servers[config[0]].held;
+            assert glb[i].ls.servers[config[0]].held;
         } else {
-            lemma_HistorySize(lb, config, i);
-            assert |lb[i].history| > 0;
-            lemma_HistoryMembership(lb, config, i);
-            assert last(lb[i].history) in lb[i].servers;
-            if exists e :: NodeAcquiresLock(e, lb[i], lb[i+1]) {
+            lemma_HistorySize(glb, config, i);
+            assert |glb[i].history| > 0;
+            lemma_HistoryMembership(glb, config, i);
+            assert last(glb[i].history) in glb[i].ls.servers;
+            /*if exists e :: NodeAcquiresLock(e, glb[i].ls, glb[i+1].ls) {
                 var e :| NodeAcquiresLock(e, lb[i], lb[i+1]);
                 assert e in AbstractifyLS_State(lb[i]).hosts;
                 assert ServiceNext(AbstractifyLS_State(lb[i]), AbstractifyLS_State(lb[i+1]));
             } else {
                 assert AbstractifyLS_State(lb[i]) == AbstractifyLS_State(lb[i+1]);
-            }
+            }*/
         }
     }
 
@@ -164,7 +184,71 @@ module RefinementProof_i {
     ///  properties needed for CorrespondenceNext
     ///////////////////////////////////////////////////////////////////
 
-    predicate NodeEpochDominates(s:LS_State, e:EndPoint, e':EndPoint)
+    lemma MakeLockHistory(glb:seq<GLS_State>, config:Config, i:int) returns (history:seq<EndPoint>)
+        requires IsValidBehavior(glb, config);
+        requires 0 <= i < |glb|-1;
+        ensures |history| > 0;
+        ensures forall p :: p in glb[i].ls.environment.sentPackets && p.msg.Transfer? && p.src in glb[i].ls.servers 
+                        ==> 2 <= p.msg.transfer_epoch <= |history|;
+        ensures forall p :: p in glb[i].ls.environment.sentPackets && p.msg.Transfer? && p.src in glb[i].ls.servers 
+                        ==> history[p.msg.transfer_epoch-1] == p.dst;
+        ensures forall h,j :: h in glb[i].ls.servers && 0 <= j < |history|-1 && history[j] == h ==> j+1 <= glb[i].ls.servers[h].epoch;
+        ensures forall h :: h in glb[i].ls.servers && h != last(history) ==> !glb[i].ls.servers[h].held;
+        ensures forall h :: h in glb[i].ls.servers && glb[i].ls.servers[h].held ==> glb[i].ls.servers[h].epoch == |history|;
+        ensures history == glb[i].history;
+        //ensures |history| > 1 ==> (forall h :: h in lb[i].servers && lb[i].servers[h].held ==> ExistsLockPacket(lb, config, i, |history|));
+        //ensures forall j :: 2 <= j < |history| ==> ExistsLockPacket(lb, config, i, j);
+        //ensures history == makeHistory(lb[i]);
+        //ensures forall epoch,h :: h in makeHistory1(lb[i])[epoch] <==> 2 <= epoch <= |history| && h == history[epoch-1];
+    {
+        if i == 0 {
+            history := [config[0]];
+        } else {
+            var prevHistory := MakeLockHistory(glb, config, i-1);
+            lemma_LS_Next(glb, config, i-1);
+            lemma_LSConsistent(glb, config, i-1);
+            lemma_LSConsistent(glb, config, i);
+            var s := glb[i-1];
+            var s' := glb[i];
+            assert LEnvironment_Next(s.ls.environment, s'.ls.environment);
+            assert forall p :: p in glb[i-1].ls.environment.sentPackets && p.msg.Locked? ==> p in glb[i].ls.environment.sentPackets;
+            /*forall j | 2 <= j < |prevHistory| 
+                ensures ExistsLockPacket(lb, config, i, j);
+            {
+                assert ExistsLockPacket(lb, config, i-1, j);
+                var p :| p in lb[i-1].environment.sentPackets && p.msg.Locked? && p.msg.locked_epoch == j;
+            }*/
+            if s.ls.environment.nextStep.LEnvStepHostIos? && s.ls.environment.nextStep.actor in s.ls.servers {
+                var id := s.ls.environment.nextStep.actor;
+                var ios := s.ls.environment.nextStep.ios;
+                
+                if NodeGrant(s.ls.servers[id], s'.ls.servers[id], ios) {
+                    if s.ls.servers[id].held && s.ls.servers[id].epoch < 0xFFFF_FFFF_FFFF_FFFF {
+                        history := prevHistory + [ios[0].s.dst];
+                    } else {
+                        history := prevHistory;
+                    }
+                } else {
+                    history := prevHistory;
+                    //assert makeHistory1(lb[i-1]) == makeHistory1(lb[i]);
+                    if   !ios[0].LIoOpTimeoutReceive? 
+                      && !s.ls.servers[id].held 
+                      && ios[0].r.src in s.ls.servers[id].config
+                      && ios[0].r.msg.Transfer? 
+                      && ios[0].r.msg.transfer_epoch > s.ls.servers[id].epoch {
+                        //history := prevHistory;
+                        var p := ios[0].r;
+                        assert IsValidLIoOp(ios[0], id, s.ls.environment);     // trigger
+                        assert p.dst == id;
+                    }
+                }
+            } else {
+                history := prevHistory;
+            }
+        }
+    }
+
+    /*predicate NodeEpochDominates(s:LS_State, e:EndPoint, e':EndPoint)
         requires e in s.servers && e' in s.servers;
     {
         s.servers[e].epoch > s.servers[e'].epoch
@@ -235,7 +319,7 @@ module RefinementProof_i {
             p.v.msg.transfer_epoch
         else 
             max(p.v.msg.transfer_epoch, servers[e.v].epoch)
-    }
+    }*/
 
 
     /*function maxEpochPacket(s:LS_State, packets:set<LockPacket>) : (LockPacket)
@@ -342,55 +426,7 @@ module RefinementProof_i {
         || (UniqueHostHoldsLock(s) && NoPacketHoldsLock(s))
     }*/
 
-    lemma MakeLockHistory(lb:seq<LS_State>, config:Config, i:int) returns (history:seq<EndPoint>)
-        requires IsValidBehavior(lb, config);
-        requires 0 <= i < |lb|-1;
-        ensures |history| > 0;
-        ensures forall p :: p in lb[i].environment.sentPackets && p.msg.Transfer? && p.src in lb[i].servers 
-                        ==> 2 <= p.msg.transfer_epoch <= |history|;
-        ensures forall p :: p in lb[i].environment.sentPackets && p.msg.Transfer? && p.src in lb[i].servers 
-                        ==> history[p.msg.transfer_epoch-1] == p.dst;
-        ensures forall h,j :: h in lb[i].servers && 0 <= j < |history|-1 && history[j] == h ==> j+1 <= lb[i].servers[h].epoch;
-        ensures forall h :: h in lb[i].servers && h != last(history) ==> !lb[i].servers[h].held;
-        ensures forall h :: h in lb[i].servers && lb[i].servers[h].held ==> lb[i].servers[h].epoch == |history|;
-    {
-        if i == 0 {
-            history := [config[0]];
-        } else {
-            var prevHistory := MakeLockHistory(lb, config, i-1);
-            lemma_LS_Next(lb, config, i-1);
-            lemma_LSConsistent(lb, config, i-1);
-            lemma_LSConsistent(lb, config, i);
-            var s := lb[i-1];
-            var s' := lb[i];
-            assert LEnvironment_Next(s.environment, s'.environment);
-            if s.environment.nextStep.LEnvStepHostIos? && s.environment.nextStep.actor in s.servers {
-                var id := s.environment.nextStep.actor;
-                var ios := s.environment.nextStep.ios;
-                if NodeGrant(s.servers[id], s'.servers[id], ios) {
-                    if s.servers[id].held && s.servers[id].epoch < 0xFFFF_FFFF_FFFF_FFFF {
-                        history := prevHistory + [ios[0].s.dst];
-                    } else {
-                        history := prevHistory;
-                    }
-                } else {
-                    history := prevHistory;
-                    if   !ios[0].LIoOpTimeoutReceive? 
-                      && !s.servers[id].held 
-                      && ios[0].r.src in s.servers[id].config
-                      && ios[0].r.msg.Transfer? 
-                      && ios[0].r.msg.transfer_epoch > s.servers[id].epoch {
-                        history := prevHistory;
-                        var p := ios[0].r;
-                        assert IsValidLIoOp(ios[0], id, s.environment);     // trigger
-                        assert p.dst == id;
-                    }
-                }
-            } else {
-                history := prevHistory;
-            }
-        }
-    }
+    //function
     /*lemma lemma_LockIsClaimedByHostOrMessage(lb:seq<LS_State>, config:Config, i:int)
         requires IsValidBehavior(lb, config);
         requires 0 <= i < |lb|-1;
