ironfleet/src/Dafny/Distributed/Services/Lock/Main.i.dfy
@@ -4,6 +4,7 @@ include "../../Common/Framework/Environment.s.dfy"
 include "../../Protocol/Common/NodeIdentity.i.dfy"
 include "../../Impl/Lock/PacketParsing.i.dfy"
 include "../../Impl/Lock/UdpLock.i.dfy"
+include "../../Impl/Lock/Host.i.dfy"
 
 module Main_i exclusively refines Main_s {
     import opened DistributedSystem_i
@@ -11,8 +12,7 @@ module Main_i exclusively refines Main_s {
     import opened Concrete_NodeIdentity_i
     import opened PacketParsing_i
     import opened UdpLock_i
-
-    type ConcreteConfiguration = Config
+    import opened Host_i
 
     predicate IsValidBehavior(config:ConcreteConfiguration, db:seq<DS_State>)
         reads *;
@@ -68,26 +68,66 @@ module Main_i exclusively refines Main_s {
                      AbstractifyConcreteEnvStep(ds_env.nextStep))
     }
 
-    
-
-    function AbstractifyConcreteConfiguration(ds_config:ConcreteConfiguration) : Config
-        //requires ConstantsStateIsValid(ds_config);
+    function AbstractifyConcreteReplicas(replicas:map<EndPoint,HostState>, replica_order:seq<EndPoint>) : map<EndPoint,Node>
+        requires forall i :: 0 <= i < |replica_order| ==> replica_order[i] in replicas;
+        requires SeqIsUnique(replica_order);
+        ensures  |AbstractifyConcreteReplicas(replicas, replica_order)| == |replica_order|;
+        ensures  forall i :: 0 <= i < |replica_order| ==> replica_order[i] in AbstractifyConcreteReplicas(replicas, replica_order);
+        ensures  forall i :: 0 <= i < |replica_order| ==> 
+                 AbstractifyConcreteReplicas(replicas, replica_order)[replica_order[i]] == replicas[replica_order[i]].node;
+        ensures forall e :: e in AbstractifyConcreteReplicas(replicas, replica_order) <==> e in replica_order;
     {
-        ds_config
+        if |replica_order| == 0 then map[]
+        else
+            lemma_UniqueSeq_SubSeqsUnique(replica_order, [replica_order[0]], replica_order[1..]);
+            assert SeqIsUnique(replica_order[1..]);
+            reveal_SeqIsUnique();
+            assert replica_order[0] !in replica_order[1..];
+            assert replica_order[0] !in AbstractifyConcreteReplicas(replicas, replica_order[1..]);
+            
+            var rest := AbstractifyConcreteReplicas(replicas, replica_order[1..]);
+            rest[replica_order[0] := replicas[replica_order[0]].node]
+    }
+
+    function AbstractifyConcreteClients(clients:set<EndPoint>) : set<NodeIdentity>
+    {
+        set e | e in clients :: e
+    }
+
+    predicate DsStateIsAbstractable(ds:DS_State) 
+    {
+           ValidConfig(ds.config)
+        && (forall r :: r in ds.config ==> r in ds.servers)
+    }
+
+    function AbstractifyDsState(ds:DS_State) : LS_State
+        requires DsStateIsAbstractable(ds);
+    {
+        LS_State(AbstractifyConcreteEnvironment(ds.environment),
+                    AbstractifyConcreteReplicas(ds.servers, ds.config))
     }
 
     lemma {:timeLimitMultiplier 2} RefinementToLSState(config:ConcreteConfiguration, db:seq<DS_State>) returns (sb:seq<LS_State>)
         requires |db| > 0;
         requires DS_Init(db[0], config);
-        requires LEnvStepIsAbstractable(last(db).environment.nextStep);
+        //requires LEnvStepIsAbstractable(last(db).environment.nextStep);
         requires forall i :: 0 <= i < |db| - 1 ==> DS_Next(db[i], db[i+1]);
         ensures  |sb| == |db|;
-        ensures  LS_Init(sb[0], AbstractifyConcreteConfiguration(db[0].config));
+        ensures  LS_Init(sb[0], db[0].config);
         ensures  forall i :: 0 <= i < |sb| - 1 ==> LS_Next(sb[i], sb[i+1]);
-        ensures forall i :: 0 <= i < |db| ==> DsStateIsAbstractable(db[i]) 
-                                           && sb[i] == AbstractifyDsState(db[i]);
-        //ensures  forall i :: 0 <= i < |db| ==> Service_Correspondence(db[i].environment.sentPackets, sb[i]);
+        ensures forall i :: 0 <= i < |db| ==> DsStateIsAbstractable(db[i]) && sb[i] == AbstractifyDsState(db[i]);
     {
+        if |db| == 1 {
+            assume false;
+            var ls := AbstractifyDsState(db[0]);
+            sb := [ ls ];
+        } else {
+        assume false;
+            var ls' := AbstractifyDsState(last(db));
+            var rest := RefinementToLSState(config, all_but_last(db));
+            //assert forall i :: 0 <= i < |rest| - 1 ==> LSHT_Next(rest[i], rest[i+1]);
+            sb := rest + [ls'];
+        }
     }
 
     lemma RefinementProofForFixedBehavior(config:ConcreteConfiguration, db:seq<DS_State>) returns (sb:seq<ServiceState>, cm:seq<int>)
