ironfleet/src/Dafny/Distributed/Impl/Lock/Node.i.dfy
@@ -3,6 +3,7 @@ include "Message.i.dfy"
 include "../Common/UdpClient.i.dfy"
 include "../../Common/Logic/Option.i.dfy"
 include "PacketParsing.i.dfy"
+include "../Common/SeqIsUniqueDef.i.dfy"
 
 module Impl_Node_i {
 import opened Protocol_Node_i
@@ -10,6 +11,7 @@ import opened Message_i
 import opened Common__UdpClient_i
 import opened Logic__Option_i
 import opened PacketParsing_i 
+import opened Common__SeqIsUniqueDef_i
 
 datatype CNode = CNode(held:bool, epoch:uint64, my_index:uint64, config:Config)
 
@@ -17,6 +19,7 @@ predicate ValidConfig(c:Config)
 {
     0 < |c| < 0x1_0000_0000_0000_0000
  && (forall e :: e in c ==> EndPointIsValidIPV4(e))
+ && SeqIsUnique(c)
 }
 
 predicate ValidConfigIndex(c:Config, index:uint64)
